ulib/FStar.Buffer.fst
@@ -9,6 +9,8 @@ open FStar.HST
 module HH = FStar.HyperHeap
 module HS = FStar.HyperStack
 
+#set-options "--initial_fuel 0 --max_fuel 0"
+
 let lemma_size (x:int) : Lemma (requires (UInt.size x n))
 				     (ensures (x >= 0))
 				     [SMTPat (UInt.size x n)]
@@ -51,20 +53,6 @@ let as_seq #a h (b:buffer a{live h b}) : GTot (seq a) = Seq.slice (sel h b) (idx
 let equal #a h (b:buffer a) h' (b':buffer a) : GTot Type0 =
   live h b /\ live h' b' /\ as_seq h b == as_seq h' b'
 
-(* Equality predicate between buffers wih quantifiers *)
-val eq_lemma: #a:Type -> h:mem -> b:buffer a{live h b} -> h':mem -> b':buffer a{live h' b'} -> Lemma
-  (requires (equal h b h' b'))
-  (ensures  (length b = length b' /\ (forall (i:nat). i < length b ==> get h b i == get h' b' i)))
-  [SMTPat (equal h b h' b')]
-let eq_lemma #a h b h' b' =
-  let s = as_seq h b in
-  let s' = as_seq h' b' in
-  assert(Seq.length s = length b);
-  assert(Seq.length s' = length b');
-  assert(Seq.equal s s');
-  assert (forall (i:nat). i < length b ==> get h b i == Seq.index s i);
-  assert (forall (i:nat). i < length b' ==> get h' b' i == Seq.index s' i)
-
 (* y is included in x / x contains y *)
 let includes #a (x:buffer a) (y:buffer a) : GTot Type0 =
   x.content == y.content /\ idx y >= idx x /\ idx x + length x >= idx y + length y
@@ -74,8 +62,8 @@ let disjoint #a #a' (x:buffer a) (y:buffer a') : GTot Type0 =
   frameOf x <> frameOf y \/ as_aref x =!= as_aref y
   \/ (as_aref x == as_aref y /\ frameOf x = frameOf y /\ (idx x + length x <= idx y \/ idx y + length y <= idx x))
 
-(* Disjointness is reflexive *)
-let lemma_disjoint_refl #a #a' (x:buffer a) (y:buffer a') : Lemma
+(* Disjointness is symmetric *)
+let lemma_disjoint_symm #a #a' (x:buffer a) (y:buffer a') : Lemma
   (requires (True))
   (ensures (disjoint x y <==> disjoint y x))
   [SMTPat (disjoint x y)]
@@ -147,6 +135,7 @@ let disjoint_from_bufs #a (b:buffer a) (bufs:TSet.set abuffer) =
 let disjoint_from_refs #a (b:buffer a) (set:TSet.set Heap.aref) =
   ~(TSet.mem (as_aref b) set)
 
+
 (* Similar but specialized disjointness predicates *)
 let disjoint_1 a b = disjoint a b
 let disjoint_2 a b b' = disjoint a b /\ disjoint a b'
@@ -163,7 +152,7 @@ let disjoint_ref_5 a r r' r'' r''' r'''' = as_aref a =!= r /\ as_aref a =!= r' /
 val disjoint_only_lemma: #a:Type -> #a':Type -> b:buffer a -> b':buffer a' -> Lemma
   (requires (disjoint b b'))
   (ensures (disjoint_from_bufs b (only b')))
-let disjoint_only_lemma #t #t' b b' = ()  
+let disjoint_only_lemma #t #t' b b' = ()
 
 (* Fully general modifies clause *)
 let modifies_bufs_and_refs (bufs:TSet.set abuffer) (refs:TSet.set Heap.aref) h h' : GTot Type0 =
@@ -171,6 +160,13 @@ let modifies_bufs_and_refs (bufs:TSet.set abuffer) (refs:TSet.set Heap.aref) h h
     (HH.modifies_rref rid (arefs bufs ++ refs) h.h h'.h
     /\ (forall (#a:Type) (b:buffer a). (frameOf b = rid /\ live h b /\ disjoint_from_bufs b bufs
       /\ disjoint_from_refs b refs) ==> equal h b h' b)))
+
+(* Fully general modifies clause for buffer sets *)
+let modifies_buffers (bufs:TSet.set abuffer) h h' : GTot Type0 =
+  (forall rid. Set.mem rid (Map.domain h.h) ==>
+    (HH.modifies_rref rid (arefs bufs) h.h h'.h /\
+      (forall (#a:Type) (b:buffer a). {:pattern (live h b /\ frameOf b = rid /\ disjoint_from_bufs b bufs)}
+	(frameOf b = rid /\ live h b /\ disjoint_from_bufs b bufs ==> equal h b h' b))))
 
 (* General modifies clause for buffers only *)
 let modifies_bufs rid buffs h h' =
@@ -203,6 +199,7 @@ let modifies_buf_4 (#t:Type) (#t':Type) (#t'':Type) (#t''':Type) rid (b:buffer t
   modifies_ref rid !{as_ref b, as_ref b', as_ref b'', as_ref b'''} h h'
   /\ (forall (#tt:Type) (bb:buffer tt). (frameOf bb = rid /\ live h bb /\ disjoint b bb /\ disjoint b' bb /\ disjoint b'' bb /\ disjoint b''' bb)
        ==> equal h bb h' bb)
+
 
 (* General lemmas for the modifies_bufs clause *)
 let lemma_modifies_bufs_trans rid bufs h0 h1 h2 :
@@ -253,6 +250,12 @@ let modifies_trans_1_1 rid b h0 h1 h2 :
   Lemma (requires (modifies_buf_1 rid b h0 h1 /\ modifies_buf_1 rid b h1 h2))
 	(ensures (modifies_buf_1 rid b h0 h2))
 	[SMTPat (modifies_buf_1 rid b h0 h1); SMTPat (modifies_buf_1 rid b h1 h2)]
+ = ()
+
+let modifies_trans_1_1' rid b b' h0 h1 h2 :
+  Lemma (requires (modifies_buf_1 rid b h0 h1 /\ modifies_buf_1 rid b' h1 h2))
+	(ensures (modifies_buf_2 rid b b' h0 h2))
+	[SMTPat (modifies_buf_1 rid b h0 h1); SMTPat (modifies_buf_1 rid b' h1 h2)]
  = ()
 
 let modifies_trans_2_0 rid b b' h0 h1 h2 :
@@ -307,8 +310,8 @@ let modifies_trans_4_4 rid b b' b'' b''' h0 h1 h2 :
 
 (* Modifies clauses that do not change the shape of the HyperStack (h1.tip = h0.tip) *)
 (* NB: those clauses are made abstract in order to make verification faster
-   It means that any missing lemma will not be provable by the programmer unless she
-   rolls back to the original 'modifies_bufs_and_refs' *)
+   Lemmas follow to allow the programmer to make use of the real definition
+   of those predicates in a general setting *)
 abstract let modifies_0 h0 h1 =
   modifies_one h0.tip h0 h1
   /\ modifies_buf_0 h0.tip h0 h1
@@ -359,6 +362,70 @@ abstract let modifies_3_2 (#a:Type) (#a':Type) (b:buffer a) (b':buffer a') h0 h1
 abstract let modifies_region rid bufs h0 h1 =
   modifies_one rid h0 h1 /\ modifies_bufs rid bufs h0 h1
 
+(* Lemmas revealing the content of the specialized modifies clauses in order to
+   be able to generalize them if needs be. *)
+let lemma_reveal_modifies_0 h0 h1 : Lemma
+  (requires (modifies_0 h0 h1))
+  (ensures  (modifies_one h0.tip h0 h1 /\ modifies_buf_0 h0.tip h0 h1 /\ h0.tip=h1.tip))
+  = ()
+
+let lemma_reveal_modifies_1 (#a:Type) (b:buffer a) h0 h1 : Lemma
+  (requires (modifies_1 b h0 h1))
+  (ensures  (let rid = frameOf b in modifies_one rid h0 h1 /\ modifies_buf_1 rid b h0 h1))
+  = ()
+
+let lemma_reveal_modifies_2_1 (#a:Type) (b:buffer a) h0 h1 : Lemma
+  (requires (modifies_2_1 b h0 h1))
+  (ensures  ( let rid = frameOf b in
+    ((rid = h0.tip /\ modifies_buf_1 rid b h0 h1 /\ modifies_one rid h0 h1)
+    \/ (rid <> h0.tip /\ HH.modifies_just (Set.union (Set.singleton rid) (Set.singleton h0.tip)) h0.h h1.h
+      /\ modifies_buf_1 rid b h0 h1 /\ modifies_buf_0 h0.tip h0 h1 ))))
+  = ()
+
+let lemma_reveal_modifies_2 (#a:Type) (#a':Type) (b:buffer a) (b':buffer a') h0 h1 : Lemma
+  (requires (modifies_2 b b' h0 h1))
+  (ensures  (let rid = frameOf b in let rid' = frameOf b' in
+    ((rid = rid' /\ modifies_buf_2 rid b b' h0 h1 /\ modifies_one rid h0 h1)
+    \/ (rid <> rid' /\ HH.modifies_just (Set.union (Set.singleton rid) (Set.singleton rid')) h0.h h1.h
+      /\ modifies_buf_1 rid b h0 h1 /\ modifies_buf_1 rid' b' h0 h1 )) ))
+  = ()
+
+let lemma_reveal_modifies_3 (#a:Type) (#a':Type) (#a'':Type) (b:buffer a) (b':buffer a')  (b'':buffer a'') h0 h1 : Lemma
+  (requires (modifies_3 b b' b'' h0 h1))
+  (ensures  (let rid = frameOf b in let rid' = frameOf b' in let rid'' = frameOf b'' in
+    ((rid = rid' /\ rid' = rid'' /\ modifies_buf_3 rid b b' b'' h0 h1 /\ modifies_one rid h0 h1)
+    \/ (rid = rid' /\ rid' <> rid'' /\ modifies_buf_2 rid b b' h0 h1 /\ modifies_buf_1 rid'' b'' h0 h1
+	/\ HH.modifies_just (Set.union (Set.singleton rid) (Set.singleton rid'')) h0.h h1.h )
+	\/ (rid <> rid' /\ rid' = rid'' /\ modifies_buf_2 rid' b' b'' h0 h1 /\ modifies_buf_1 rid b h0 h1
+	/\ HH.modifies_just (Set.union (Set.singleton rid) (Set.singleton rid'')) h0.h h1.h )
+	\/ (rid = rid'' /\ rid' <> rid'' /\ modifies_buf_2 rid b b'' h0 h1 /\ modifies_buf_1 rid' b' h0 h1
+	/\ HH.modifies_just (Set.union (Set.singleton rid) (Set.singleton rid')) h0.h h1.h )
+	\/ (rid <> rid' /\ rid' <> rid'' /\ rid <> rid''
+	/\ HH.modifies_just (Set.union (Set.union (Set.singleton rid) (Set.singleton rid')) (Set.singleton rid'')) h0.h h1.h
+	/\ modifies_buf_1 rid b h0 h1 /\ modifies_buf_1 rid' b' h0 h1 /\ modifies_buf_1 rid'' b'' h0 h1)) ))
+  = ()
+
+let lemma_reveal_modifies_3_2 (#a:Type) (#a':Type) (b:buffer a) (b':buffer a') h0 h1 : Lemma
+  (requires (modifies_3_2 b b' h0 h1))
+  (ensures  (let rid = frameOf b in let rid' = frameOf b' in
+    ((rid = rid' /\ rid' = h0.tip /\ modifies_buf_2 rid b b' h0 h1 /\ modifies_one rid h0 h1)
+    \/ (rid = rid' /\ rid' <> h0.tip /\ modifies_buf_2 rid b b' h0 h1 /\ modifies_buf_0 h0.tip h0 h1
+      /\ HH.modifies_just (Set.union (Set.singleton rid) (Set.singleton h0.tip)) h0.h h1.h )
+      \/ (rid <> rid' /\ rid = h0.tip /\ modifies_buf_1 rid b h0 h1 /\ modifies_buf_1 rid' b' h0 h1
+	/\ HH.modifies_just (Set.union (Set.singleton rid') (Set.singleton h0.tip)) h0.h h1.h )
+	\/ (rid <> rid' /\ rid' = h0.tip /\ modifies_buf_1 rid' b' h0 h1 /\ modifies_buf_1 rid b h0 h1
+	/\ HH.modifies_just (Set.union (Set.singleton rid) (Set.singleton h0.tip)) h0.h h1.h )
+	\/ (rid <> rid' /\ rid' <> h0.tip /\ rid <> h0.tip
+	/\ HH.modifies_just (Set.union (Set.union (Set.singleton rid) (Set.singleton rid')) (Set.singleton h0.tip)) h0.h h1.h
+	/\ modifies_buf_1 rid b h0 h1 /\ modifies_buf_1 rid' b' h0 h1 /\ modifies_buf_0 h0.tip h0 h1)) ))
+  = ()
+
+let lemma_reveal_modifies_region rid bufs h0 h1 : Lemma
+  (requires (modifies_region rid bufs h0 h1))
+  (ensures  (modifies_one rid h0 h1 /\ modifies_bufs rid bufs h0 h1))
+  = ()
+
+
 (* STStack effect specific lemmas *)
 let lemma_ststack_1 (#a:Type) (b:buffer a) h0 h1 h2 h3 : Lemma
   (requires (live h0 b /\ fresh_frame h0 h1 /\ modifies_1 b h1 h2 /\ popped h2 h3))
@@ -395,7 +462,7 @@ let lemma_modifies_3_2_comm (#a:Type) (#a':Type) (b:buffer a) (b':buffer a') h0 
   = ()
 (* TODO: add commutativity lemmas for modifies_3 *)
 
-#reset-options
+#reset-options "--initial_fuel 0 --max_fuel 0 --z3timeout 20"
 
 (** Transitivity lemmas *)
 let lemma_modifies_0_trans h0 h1 h2 : Lemma
@@ -431,7 +498,7 @@ let lemma_modifies_2_trans' (#a:Type) (#a':Type) (b:buffer a) (b':buffer a') h0 
   [SMTPat (modifies_2 b' b h0 h1); SMTPatT (modifies_2 b b' h1 h2)]
   = ()
 
-#reset-options "--z3timeout 20"
+#reset-options "--z3timeout 20 --initial_fuel 0 --max_fuel 0"
 #set-options "--lax" // OK
 
 let lemma_modifies_3_trans (#a:Type) (#a':Type) (#a'':Type) (b:buffer a) (b':buffer a') (b'':buffer a'') h0 h1 h2 : Lemma
@@ -467,7 +534,7 @@ val lemma_modifies_0_0: h0:mem -> h1:mem -> h2:mem -> Lemma
   [SMTPat (modifies_0 h0 h1); SMTPat (modifies_0 h1 h2)]
 let lemma_modifies_0_0 h0 h1 h2 = ()
 
-#reset-options "--z3timeout 20"
+#reset-options "--initial_fuel 0 --max_fuel 0 --z3timeout 20"
 
 let lemma_modifies_1_0 (#a:Type) (b:buffer a) h0 h1 h2 : Lemma
   (requires (live h0 b /\ live h1 b /\ modifies_1 b h0 h1 /\ modifies_0 h1 h2))
@@ -487,7 +554,7 @@ let lemma_modifies_0_1' (#a:Type) (b:buffer a) h0 h1 h2 : Lemma
   [SMTPat (modifies_0 h0 h1); SMTPat (modifies_1 b h1 h2)]
   = ()
 
-#reset-options "--z3timeout 100"
+#reset-options "--initial_fuel 0 --max_fuel 0 --z3timeout 100"
 
 let lemma_modifies_1_1 (#a:Type) (#a':Type) (b:buffer a) (b':buffer a') h0 h1 h2 : Lemma
   (requires (live h0 b /\ live h0 b' /\ disjoint b b'
@@ -557,36 +624,15 @@ let lemma_modifies_2_1' (#a:Type) (#a':Type) (b:buffer a) (b':buffer a') h0 h1 h
   [SMTPat (modifies_2 b' b h0 h1); SMTPat (modifies_1 b h1 h2)]
   = ()
 
+let lemma_modifies_2_1'' (#a:Type) (#a':Type) (b:buffer a) (b':buffer a') h0 h1 h2 : Lemma
+  (requires (live h0 b /\ live h0 b' /\ disjoint b b' /\ modifies_2_1 b h0 h1 /\ modifies_1 b' h1 h2))
+  (ensures  (modifies_3_2 b b' h0 h2))
+  [SMTPat (modifies_2_1 b h0 h1); SMTPat (modifies_1 b' h1 h2)]
+  = ()
+
 (* TODO: lemmas for modifies_3 *)
 
-#reset-options
-
-(* (\* Axiomatization issue with 'arefs' *\) *)
-(* let lemma_modifies_buf_0 (#a:Type) (b:buffer a) h0 h1 h2 : Lemma *)
-(*   (requires (~(contains h0 b) /\ live h1 b /\ modifies_bufs (frameOf b) !{} h0 h1 *)
-(*     /\ modifies_bufs (frameOf b) ((only b)) h1 h2)) *)
-(*   (ensures (modifies_bufs (frameOf b) !{} h0 h2)) *)
-(*   = let rid = frameOf b in *)
-(*     let h = Map.sel h0.h rid in *)
-(*     let h' = Map.sel h1.h rid in *)
-(*     let h'' = Map.sel h2.h rid in *)
-(*     cut (Heap.modifies !{} h h'); *)
-(*     cut (Heap.modifies (arefs (!! (Buff b))) h' h''); *)
-(*     assert(modifies_bufs (frameOf b) TSet.empty h0 h1); *)
-(*     assert(modifies_bufs (frameOf  *)
-(*     assert(modifies_bufs (frameOf b) (!! (Buff b)) h0 h1); admit() *)
-(*     assert(TSet.equal (arefs (TSet.union empty (TSet.singleton (Buff b)))) *)
-(* 		     (TSet.union (arefs TSet.empty) (TSet.singleton (as_aref b))) ); *)
-(*     assert(TSet.equal (TSet.union empty (TSet.singleton (Buff b))) (only b)); *)
-(*     TSet.lemma_equal_intro (arefs (only b)) !{as_ref b} *)
-
-(* #reset-options *)
-
-(* val lemma_modifies_fresh_2: #t:Type -> #t':Type -> a:buffer t -> b:buffer t' -> h0:mem -> h1:mem -> Lemma *)
-(*   (requires (~(contains h0 b) /\ live h1 b /\ frameOf b = h0.tip /\ modifies_2 a b h0 h1)) *)
-(*   (ensures (~(contains h0 b) /\ live h1 b /\ frameOf b = h0.tip *)
-(*     /\ modifies_buf_1 (frameOf a) a h0 h1 )) *)
-(* let lemma_modifies_fresh_2 #t #t' a b h0 h1 = () *)
+#reset-options "--initial_fuel 0 --max_fuel 0"
 
 (** Concrete getters and setters *)
 let create #a (init:a) (len:UInt32.t) : ST (buffer a)
@@ -680,8 +726,6 @@ val upd: #a:Type -> b:buffer a -> n:UInt32.t -> z:a -> STL unit
   (ensures (fun h0 _ h1 -> live h0 b /\ live h1 b /\ v n < length b
     /\ modifies_1 b h0 h1
     /\ as_seq h1 b == Seq.upd (as_seq h0 b) (v n) z ))
-    (* /\ get h1 b (v n) == z *)
-    (* /\ (forall (i:nat). {:pattern (get h1 b i)} (i < length b /\ i <> v n) ==> get h1 b i == get h0 b i) *)
 let upd #a b n z =
   let s0 = !b.content in
   let s = Seq.upd s0 (v b.idx + v n) z in
@@ -693,32 +737,35 @@ let upd #a b n z =
   ()
 
 (* Could be made Total with a couple changes in the spec *)
-let sub #a (b:buffer a) (i:UInt32.t) (len:UInt32.t{v len <= length b /\ v i + v len <= length b}) : STL (buffer a)
-     (requires (fun h -> live h b))
-     (ensures (fun h0 b' h1 -> content b == content b' /\ idx b' = idx b + v i /\ length b' = v len
-       /\ h0 == h1 /\ includes b b' /\ live h1 b' /\ live h0 b
-       /\ as_seq h1 b' == Seq.slice (as_seq h0 b) (v i) (v i + v len) ))
-  = let b' = {content = b.content; idx = i +^ b.idx; length = len} in
-    let h = HST.get() in
-    Seq.lemma_eq_intro (as_seq h b') (Seq.slice (as_seq h b) (v i) (v i + v len));
-    b'
+let sub #a (b:buffer a) (i:UInt32.t{v i + v b.idx < pow2 n}) (len:UInt32.t{v len <= length b /\ v i + v len <= length b}) : Tot (b':buffer a{b `includes` b'})
+  = {content = b.content; idx = i +^ b.idx; length = len}
 
-let offset #a (b:buffer a) (i:UInt32.t{v i <= length b}) : STL (buffer a)
-  (requires (fun h -> live h b))
-  (ensures (fun h0 b' h1 -> content b' == content b /\ idx b' = idx b + v i /\ length b' = length b - v i
-    /\ h0 == h1 /\ includes b b' /\ live h1 b'
-    /\ as_seq h1 b' == Seq.slice (as_seq h0 b) (v i) (length b) ))
-  = let b' = {content = b.content; idx = i +^ b.idx; length = b.length -^ i} in
-    let h = HST.get() in
-    Seq.lemma_eq_intro (as_seq h b') (Seq.slice (as_seq h b) (v i) (length b));
-    b'
+let lemma_sub_spec (#a:Type) (b:buffer a)
+  (i:UInt32.t{v i + v b.idx < pow2 n})
+  (len:UInt32.t{v len <= length b /\ v i + v len <= length b})
+  h : Lemma
+     (requires (live h b))
+     (ensures  (live h b /\ as_seq h (sub b i len) == Seq.slice (as_seq h b) (v i) (v i + v len)))
+     [SMTPat (sub b i len); SMTPat (live h b)]
+  = Seq.lemma_eq_intro (as_seq h (sub b i len)) (Seq.slice (as_seq h b) (v i) (v i + v len))
+
+let offset #a (b:buffer a) (i:UInt32.t{v i + v b.idx < pow2 n /\ v i <= v b.length}) : Tot (b':buffer a{b `includes` b'})
+  = {content = b.content; idx = i +^ b.idx; length = b.length -^ i}
+
+let lemma_offset_spec (#a:Type) (b:buffer a)
+  (i:UInt32.t{v i + v b.idx < pow2 n /\ v i <= v b.length})
+  h : Lemma
+     (requires (live h b))
+     (ensures  (live h b /\ as_seq h (offset b i) == Seq.slice (as_seq h b) (v i) (length b)))
+     [SMTPat (offset b i); SMTPat (live h b)]
+  = Seq.lemma_eq_intro (as_seq h (offset b i)) (Seq.slice (as_seq h b) (v i) (length b))
 
 (**
     Defining operators for buffer accesses as specified at
     https://github.com/FStarLang/FStar/wiki/Parsing-and-operator-precedence
    *)
-(* (\** JP: if the [val] is not specified, there's an issue with these functions *)
-(*  * taking an extra unification parameter at extraction-time... *\) *)
+(* JP: if the [val] is not specified, there's an issue with these functions
+ * taking an extra unification parameter at extraction-time... *)
 val op_Array_Access: #a:Type -> b:buffer a -> n:UInt32.t{v n<length b} -> STL a
      (requires (fun h -> live h b))
      (ensures (fun h0 z h1 -> live h0 b /\ h1 == h0
@@ -738,65 +785,25 @@ let lemma_modifies_one_trans_1 (#a:Type) (b:buffer a) (h0:mem) (h1:mem) (h2:mem)
   [SMTPat (modifies_one (frameOf b) h0 h1); SMTPat (modifies_one (frameOf b) h1 h2)]
   = ()
 
-#reset-options "--z3timeout 100"
-#set-options "--lax" // TODO: restore after switching to FStar.Seq-based specification
-
-private val blit_aux: #a:Type -> b:buffer a -> idx_b:UInt32.t ->
-  b':buffer a -> idx_b':UInt32.t -> len:UInt32.t{v idx_b+v len<=length b/\v idx_b'+v len<= length b'} ->
-  ctr:UInt32.t{v ctr <= v len} ->  STL unit
-  (requires (fun h -> live h b /\ live h b' /\ disjoint b b'
-    /\ (forall (i:nat). i < v ctr ==> get h b (v idx_b+i) == get h b' (v idx_b'+i)) ))
-  (ensures (fun h0 _ h1 -> live h1 b /\ live h1 b'  /\ live h0 b /\ live h0 b'
-    /\ disjoint b b' /\ length b >= v idx_b+v len /\ length b' >= v idx_b'+v len
-    /\ modifies_1 b' h0 h1
-    /\ (forall (i:nat). {:pattern (get h1 b' (v idx_b'+i))} i < v len
-	==> get h0 b (v idx_b+i) == get h1 b' (v idx_b'+i))
-    /\ (forall (i:nat). {:pattern (get h1 b' i)} (i < v idx_b' \/ (i >= v idx_b'+v len /\ i < length b'))
-	==> get h1 b' i == get h0 b' i) ))
-let rec blit_aux #a b idx_b b' idx_b' len ctr =
-  let h0 = HST.get() in
-  if (len -^ ctr) =^ (uint_to_t 0) then ()
-  else
-  begin
-    let bctr = index b (idx_b +^ ctr) in
-    upd b' (idx_b' +^ ctr) bctr;
-    blit_aux b idx_b b' idx_b' len (ctr +^ (uint_to_t 1))
-  end
-
-#reset-options
-#set-options "--lax"
-
-val blit: #t:Type -> a:buffer t -> idx_a:UInt32.t{v idx_a <= length a} -> b:buffer t{disjoint a b} -> 
+(* JK: TODO, corresponds to memcpy *)
+assume val blit: #t:Type -> a:buffer t -> idx_a:UInt32.t{v idx_a <= length a} -> b:buffer t{disjoint a b} ->
   idx_b:UInt32.t{v idx_b <= length b} -> len:UInt32.t{v idx_a+v len <= length a /\ v idx_b+v len <= length b} -> STL unit
     (requires (fun h -> live h a /\ live h b))
     (ensures (fun h0 _ h1 -> live h0 b /\ live h0 a /\ live h1 b /\ live h1 a
-      (* /\ (forall (i:nat). {:pattern (get h1 b (v idx_b+i))} i < v len ==> get h1 b (v idx_b+i) == get h0 a (v idx_a+i)) *)
-      (* /\ (forall (i:nat). {:pattern (get h1 b i)} ((i >= v idx_b + v len /\ i < length b) \/ i < v idx_b) ==> get h1 b i == get h0 b i) *)
       /\ Seq.slice (as_seq h1 b) (v idx_b) (v idx_b+v len) == Seq.slice (as_seq h0 a) (v idx_a) (v idx_a+v len)
       /\ Seq.slice (as_seq h1 b) 0 (v idx_b) == Seq.slice (as_seq h0 b) 0 (v idx_b)
       /\ Seq.slice (as_seq h1 b) (v idx_b+v len) (length b) == Seq.slice (as_seq h0 b) (v idx_b+v len) (length b)
       /\ modifies_1 b h0 h1 ))
-let blit #t a idx_a b idx_b len = blit_aux a idx_a b idx_b len (uint_to_t 0)
 
-#reset-options
-
+(* JK: TODO, corresponds to memset *)
 assume val fill: #t:Type -> b:buffer t -> z:t -> len:UInt32.t{v len <= length b} -> STL unit
   (requires (fun h -> live h b))
   (ensures  (fun h0 _ h1 -> live h0 b /\ live h1 b /\ modifies_1 b h0 h1
     /\ Seq.slice (as_seq h1 b) 0 (v len) == Seq.create (v len) z
     /\ Seq.slice (as_seq h1 b) (v len) (length b) == Seq.slice (as_seq h0 b) (v len) (length b) ))
 
-#reset-options
-
-val split: #a:Type -> a:buffer t -> i:UInt32.t{v i <= length a} -> STL (buffer t * buffer t)
-    (requires (fun h -> live h a))
-    (ensures (fun h0 b h1 -> live h1 (fst b) /\ live h1 (snd b) /\ h1 == h0 /\ idx (fst b) = idx a
-      /\ idx (snd b) = idx a + v i /\ length (fst b) = v i /\ length (snd b) = length a - v i
-      /\ disjoint (fst b) (snd b)  /\ content (fst b) == content a /\ content (snd b) == content a
-      /\ as_seq h1 (fst b) == Seq.slice (as_seq h0 a) 0 (v i)
-      /\ as_seq h1 (snd b) == Seq.slice (as_seq h0 a) (v i) (length a) ))
-let split #t a i =
-  let a1 = sub a (uint_to_t 0) i in let a2 = sub a i (a.length -^ i) in a1, a2
+let split #t (b:buffer t) (i:UInt32.t{v i <= length b /\ v i + v b.idx < pow2 n}) : Tot (buffer t * buffer t)
+  = sub b 0ul i, offset b i
 
 val no_upd_lemma_0: #t:Type -> h0:mem -> h1:mem -> b:buffer t -> Lemma
   (requires (live h0 b /\ modifies_0 h0 h1))
@@ -810,7 +817,7 @@ val no_upd_lemma_1: #t:Type -> #t':Type -> h0:mem -> h1:mem -> a:buffer t -> b:b
   [SMTPat (modifies_1 a h0 h1); SMTPat (live h0 b)]
 let no_upd_lemma_1 #t #t' h0 h1 a b = ()
 
-#reset-options "--z3timeout 30"
+#reset-options "--z3timeout 30 --initial_fuel 0 --max_fuel 0"
 
 val no_upd_lemma_2: #t:Type -> #t':Type -> #t'':Type -> h0:mem -> h1:mem -> a:buffer t -> a':buffer t' -> b:buffer t'' -> Lemma
   (requires (live h0 b /\ disjoint a b /\ disjoint a' b /\ modifies_2 a a' h0 h1))
@@ -835,39 +842,6 @@ val no_upd_popped: #t:Type -> h0:mem -> h1:mem -> b:buffer t -> Lemma
   (ensures  (live h0 b /\ live h1 b /\ equal h0 b h1 b))
   [SMTPat (live h0 b); SMTPat (popped h0 h1)]
 let no_upd_popped #t h0 h1 b = ()
-
-let eq_lemma_0 (#t:Type) h0 h1 (b:buffer t) : Lemma
-  (requires (modifies_0 h0 h1 /\ live h0 b))
-  (ensures  (live h0 b /\ live h1 b /\ (forall (i:nat). {:pattern (get h1 b i)} i < length b ==> get h1 b i == get h0 b i) ))
-  = ()
-
-let eq_lemma_1 (#t:Type) (#t':Type) h0 h1 (a:buffer t) (b:buffer t') : Lemma
-  (requires (modifies_1 a h0 h1 /\ disjoint a b /\ live h0 b))
-  (ensures  (live h0 b /\ live h1 b /\ (forall (i:nat). {:pattern (get h1 b i)} i < length b
-					       ==> get h1 b i == get h0 b i)))
-  = ()
-
-let eq_lemma_2 (#t:Type) (#t':Type) (#t'':Type) h0 h1 (a:buffer t) (a':buffer t') (b:buffer t'') : Lemma
-  (requires (modifies_2 a a' h0 h1 /\ disjoint a b /\ disjoint a' b /\ live h0 b))
-  (ensures  (live h0 b /\ live h1 b /\ (forall (i:nat). {:pattern (get h1 b i)} i < length b ==> get h1 b i == get h0 b i)))
-  = ()
-
-let eq_lemma_2_1 (#t:Type) (#t':Type) h0 h1 (b:buffer t) (b':buffer t) : Lemma
-  (requires (modifies_2_1 b h0 h1 /\ live h0 b' /\ disjoint b b'))
-  (ensures  (live h0 b' /\ live h1 b' /\ (forall (i:nat). {:pattern (get h1 b i)} i < length b' ==> get h1 b' i == get h0 b' i) ))
-  = ()
-
-let eq_lemma_fresh h0 h1 a : Lemma
-  (requires (live h0 a /\ fresh_frame h0 h1))
-  (ensures  (live h0 a /\ live h1 a /\ (forall (i:nat). {:pattern (get h1 a i)} i < length a
-			    ==> get h1 a i == get h0 a i)))
-  = ()
-
-val eq_lemma_popped: #t:Type -> h0:mem -> h1:mem -> b:buffer t -> Lemma
-  (requires (live h0 b /\ frameOf b <> h0.tip /\ popped h0 h1))
-  (ensures  (live h0 b /\ live h1 b
-    /\ (forall (i:nat). {:pattern (get h1 b i)} i < length b ==> get h1 b i == get h0 b i)))
-let eq_lemma_popped #t h0 h1 b = ()
 
 (* Modifies of subset lemmas *)
 let lemma_modifies_sub_0 h0 h1 : Lemma
@@ -894,7 +868,7 @@ let lemma_modifies_sub_2_1 #t h0 h1 (b:buffer t) : Lemma
   [SMTPat (live h0 b); SMTPat (modifies_2_1 b h0 h1)]
   = ()
 
-#reset-options "--z3timeout 100"
+#reset-options "--z3timeout 100 --initial_fuel 0 --max_fuel 0"
 
 (* TODO *)
 let modifies_subbuffer_1 (#t:Type) h0 h1 (sub:buffer t) (a:buffer t) : Lemma
@@ -927,6 +901,12 @@ let modifies_subbuffer_2_prime (#t:Type) h0 h1 (sub1:buffer t) (sub2:buffer t) (
   (requires (live h0 a /\ includes a sub1 /\ includes a sub2 /\ modifies_2 sub1 sub2 h0 h1))
   (ensures  (modifies_1 a h0 h1 /\ live h1 a))
   [SMTPat (modifies_2 sub1 sub2 h0 h1); SMTPat (includes a sub1); SMTPat (includes a sub2)]
+  = ()
+
+let modifies_popped_3_2 (#t:Type) #t' (a:buffer t) (b:buffer t') h0 h1 h2 h3 : Lemma
+  (requires (live h0 a /\ live h0 b /\ fresh_frame h0 h1 /\ popped h2 h3 /\ modifies_3_2 a b h1 h2))
+  (ensures  (modifies_2 a b h0 h3))
+  [SMTPat (fresh_frame h0 h1); SMTPat (popped h2 h3); SMTPat (modifies_3_2 a b h1 h2)]
   = ()
 
 let modifies_popped_2 (#t:Type) #t' (a:buffer t) (b:buffer t') h0 h1 h2 h3 : Lemma
